more

coq/Logic/Axiom/Reduction.v
@@ -1,9 +1,16 @@
 Require Import Logic.Axiom.Dec.
+Require Import Logic.Axiom.Sec.
+Require Import Logic.Axiom.Sat.
 
 Definition red (a b:Type) (p:a -> Prop) (q:b -> Prop) (f:a -> b) : Prop :=
    forall (x:a), p x <-> q (f x). 
 
 Arguments red {a} {b}.
+
+Definition ReducesTo (a b:Type) (p:a -> Prop) (q:b -> Prop) : Prop :=
+    exists (f:a -> b), red p q f.
+
+Arguments ReducesTo {a}{b}. 
 
 Lemma redDec : forall (a b:Type) (p:a -> Prop) (q:b -> Prop) (f:a -> b),
     red p q f -> pDec q -> pDec p.
@@ -15,4 +22,36 @@ Proof.
     - right. intros H4. apply H2, H1. assumption.
 Qed.
 
+Lemma ReducesDecidable : forall (a b:Type) (p:a -> Prop) (q:b -> Prop),
+    ReducesTo p q -> Decidable q -> Decidable p.
+Proof.
+    intros a b p q [f H1] [g H2]. exists (fun n => g (f n)). intros x.
+    unfold red in H1. specialize H1 with x.
+    unfold DeciderOf in H2. specialize H2 with (f x).
+    destruct H1 as [H1 G1]. destruct H2 as [H2 G2]. split; intros H3.
+    - apply H2, H1, H3.
+    - apply G1, G2, H3.
+Qed.
+
+Lemma redSec : forall (a b:Type) (p:a -> Prop) (q:b -> Prop) (f:a -> b),
+    red p q f -> pSec q -> pSec p.
+Proof.
+    intros a b p q f H1 H2 x. unfold pSec in H2.
+    unfold red in H1. specialize H1 with x. destruct H1 as [H1 H3].
+    specialize H2 with (f x). destruct H2 as [g H2].
+    exists g. destruct H2 as [H2 H4]. split; intros H5.
+    - apply H2, H1, H5.
+    - apply H3, H4, H5.
+Qed.
+
+Lemma ReducesSemiDecidable : forall (a b:Type) (p:a -> Prop) (q:b -> Prop),
+    ReducesTo p q -> SemiDecidable q -> SemiDecidable p.
+Proof.
+    intros a b p q [f H1] [F H2]. exists (fun x n => F (f x) n). intros x.
+    unfold red in H1. specialize H1 with x.
+    unfold SemiDeciderOf in H2. specialize H2 with (f x).
+    destruct H1 as [H1 G1]. destruct H2 as [H2 G2]. split; intros H3.
+    - apply H2, H1, H3.
+    - apply G1, G2, H3.
+Qed.
 
