coq/Logic/Lang1/Incl.v
@@ -7,8 +7,12 @@ Require Import Logic.Set.Incl.
 Require Import Logic.Set.Equal.
 
 Require Import Logic.Lang1.Syntax.
+Require Import Logic.Lang1.Context.
+Require Import Logic.Lang1.SemanCtx.
 Require Import Logic.Lang1.Semantics.
 Require Import Logic.Lang1.Environment.
+
+Open Scope Set_Incl_scope.
 
 (* Lemma 'inclRefl' expressed in set theory abstract syntax.                    *)
 Definition inclReflF (n:nat) : Formula := All n (Sub n n).
@@ -24,10 +28,11 @@ Definition inclReflF (n:nat) : Formula := All n (Sub n n).
 (* With this caveat in mind, we assert that evaluating inclReflF in any         *)
 (* environment (and for any choice of variable name 'n') yields a proposition   *)
 (* which is equivalent to the lemma inclRefl.                                   *)
-Lemma evalInclReflF : LEM -> forall (e:Env) (n:nat),
+Import Semantics.
+Lemma evalInclReflF : forall (e:Env) (n:nat),
     eval e (inclReflF n) <-> forall (x:set), x <= x.
 Proof.
-    intros L e n. unfold inclReflF. rewrite evalAll. split; intros H x.
+    intros e n. unfold inclReflF. rewrite evalAll. split; intros H x.
     - remember (H x) as H' eqn:E. clear E. 
       rewrite evalSub in H'. 
         + rewrite bindSame in H'. assumption.
@@ -35,19 +40,29 @@ Proof.
         + rewrite bindSame. apply H.
 Qed.        
 
+Import SemanCtx.
+Lemma evalInclReflFCtx : forall (G:Context) (n:nat),
+    G :- (inclReflF n) >> forall (x:set), x <= x.
+Proof.
+    intros G n. unfold inclReflF.
+    apply evalAll. intros x. apply evalSub; apply FindZ.
+Qed.
+ 
+
 (* An approximation of lemma 'inclNil' expressed in set theory abstract syntax. *)
 (* This formulation is correct when variables n and m are distinct.             *)
 Definition inclNilF (n m:nat) : Formula := 
     All n (Imp (Empty n) (All m (Sub n m))).
 
+Import Semantics.
 (* Evaluating  inclNilF in any environment 'yields' the lemma inclNil.          *)
-Lemma evalInclNilF : LEM -> forall (e:Env) (n m:nat), 
+Lemma evalInclNilF : forall (e:Env) (n m:nat), 
     m <> n ->
     eval e (inclNilF n m ) 
         <-> 
     forall (x:set), x == Nil -> forall (y:set), x <= y.
 Proof.
-    intros L e n m Hmn. unfold inclNilF. rewrite evalAll. split; intros H x.
+    intros e n m Hmn. unfold inclNilF. rewrite evalAll. split; intros H x.
     - remember (H x) as H' eqn:E. clear E H. rewrite evalImp in H'.
       rewrite evalEmpty in H'. rewrite bindSame in H'. intro H.
       remember (H' H) as H0 eqn:E. clear E H H'. rewrite evalAll in H0.
@@ -62,3 +77,15 @@ Proof.
         + assumption.
 Qed.
 
+Import SemanCtx.
+Lemma evalInclNilFCtx : LEM -> forall (G:Context) (n m:nat), 
+    n <> m ->
+    G :- (inclNilF n m )  >>
+        forall (x:set), x == Nil -> forall (y:set), x <= y.
+Proof.
+    intros L G n m H1. unfold inclNilF.
+    apply evalAll. intros x. apply evalImp.
+    - apply evalEmpty, FindZ.
+    - apply evalAll. intros y. apply evalSub; try (apply FindZ).
+      apply FindS; try assumption. apply FindZ.
+Qed.
