lean/tutorials/tutorial7.lean
@@ -1,0 +1,26 @@
+import tuto_lib
+import data.int.parity
+
+
+example : false → 0 = 1 :=
+begin
+  intros H₁, exfalso, assumption
+end
+
+example : ∀ (x : ℝ), ¬ x < x :=
+begin
+  intros x H₁, rw lt_iff_le_and_ne at H₁, cases H₁ with H₁ H₂, clear H₁,
+  change x = x → false at H₂, apply H₂, refl
+end
+
+open int
+
+example : ∀ (n : ℤ), even n → ¬ even n → 0 = 1 :=
+begin
+  intros n H₁ H₂, exfalso, apply H₂, assumption
+end
+
+example : ∀ (P Q:Prop), (P ∨ Q) → ¬(P ∧ Q) → ¬ P ↔ Q :=
+begin
+  intros P Q, intros H₁,
+end
